ems/ModSemFacts.v
@@ -34,7 +34,7 @@ Module ModSemFacts.
 Import ModSem.
 Section COMM.
 
-  (* TODO: Current definition of module linking is not commutative. (add ms1 ms2).(init_st) ≠ (add ms2 ms1).(init_st) *)
+  (* TODO: Current definition of module linking is not commutative. (add ms1 ms2).(initial_st) ≠ (add ms2 ms1).(initial_st) *)
 
   Inductive comm_emb : IFun Es Es -> IFun Es Es -> Prop := 
     |comm_emb_1 : comm_emb emb_l emb_r
@@ -133,6 +133,7 @@ Section COMM.
   <<COMM: Beh.of_program (compile (add ms0 ms1) (Some P0)) <1= Beh.of_program (compile (add ms1 ms0) (Some P1))>>
   .
   Proof.
+  Admitted.
     (* destruct (classic (P1)); cycle 1.
     { ii. eapply initial_itr_not_wf;et. }
     replace P0 with P1.
@@ -183,13 +184,10 @@ Section COMM.
         * unfold sim_fsem, "==>". i. eapply add_comm_aux; et.
           rewrite H0. econs. econs.
       + left. unfold trans_l, trans_r.
-        rewrite ! alist_find_map. rewrite MS1, MS0. et. *)
+        rewrite ! alist_find_map. rewrite MS1, MS0. et.
 
-    (* - exists tt. econs; et; clarify.
-      unfold comm_st. ss. exists (init_st ms1), (init_st ms0). et. *)
-
-      Admitted.
-(* Qed. *)
+    - (* initial_st has 'Take' only *) admit.
+Qed. *)
 
 End COMM.
 Section ASSOC.
@@ -418,7 +416,7 @@ Proof.
   eapply adequacy_local_aux; et.
 
   (* 2: { exists tt. instantiate (1:= top2). instantiate (1:=(fun _ => assoc_st)).  econs; et; clarify. 
-       unfold assoc_st. ss. exists (init_st ms0), (init_st ms1), (init_st ms2). splits; et. } *)
+       unfold assoc_st. ss. exists (initial_st ms0), (initial_st ms1), (initial_st ms2). splits; et. } *)
   (* { admit. }
   i. s.
   unfold add_fnsems, trans_l, trans_r. s. unfold add_fnsems, trans_l, trans_r. 
@@ -501,7 +499,7 @@ Proof.
   unfold compile. red. 
   eapply adequacy_local_aux; et.
   (* 2: { exists tt. instantiate (1:= top2). instantiate (1:=(fun _ => assoc_rev_st)).  econs; et; clarify. 
-       unfold assoc_rev_st. ss. exists (init_st ms0), (init_st ms1), (init_st ms2). splits; et. } *)
+       unfold assoc_rev_st. ss. exists (initial_st ms0), (initial_st ms1), (initial_st ms2). splits; et. } *)
   { admit. }
   i. s.
   unfold add_fnsems, trans_l, trans_r. s. unfold add_fnsems, trans_l, trans_r. 
@@ -677,7 +675,7 @@ Admitted.
   unfold compile. red. 
   eapply adequacy_local_aux; et.
   2: { exists tt. instantiate (1:= top2). instantiate (1:= (fun _ => empty_st)). econs; et; clarify.
-       unfold empty_st. ss. exists (init_st ms). et. }
+       unfold empty_st. ss. exists (initial_st ms). et. }
   i. s.
   unfold add_fnsems, trans_l, trans_r. s.
   rewrite ! alist_find_app_o. rewrite ! alist_find_map. 
@@ -705,7 +703,7 @@ Admitted.
   unfold compile. red. 
   eapply adequacy_local_aux; et.
   2: { exists tt. instantiate (1:= top2). instantiate (1:= (fun _ => empty_rev_st)). econs; et; clarify.
-       unfold empty_st. ss. exists (init_st ms). et. }
+       unfold empty_st. ss. exists (initial_st ms). et. }
   i. s.
   unfold add_fnsems, trans_l, trans_r. s.
   rewrite ! alist_find_app_o. rewrite ! alist_find_map. 
@@ -936,9 +934,9 @@ Proof. ss. destruct xs; ss. Qed.
 
   Lemma add_list_initial_mrs (mdl: list t) (ske: Sk.t)
      :
-       ModSem.init_st (Mod.get_modsem (add_list mdl) ske)
+       ModSem.initial_st (Mod.get_modsem (add_list mdl) ske)
        =
-       add_mrs_list ((List.map (fun md => ModSem.init_st (get_modsem md ske)) mdl)).
+       add_mrs_list ((List.map (fun md => ModSem.initial_st (get_modsem md ske)) mdl)).
    Proof.
      induction mdl; ss.
      destruct mdl; ss.
